semantics: Refactor definitions and soundness for isL

theories/Semantics/IntuitionisticKripkeSemantics.v
@@ -5,63 +5,89 @@ Require Import Formulas Sequents.
 
 (* Source: A New Calculus for Intuitionistic Strong Löb Logic *)
 
-(* for iSL *)
-(* TODO: give names *)
-Class IntuitionisticModalKripkeModel
-  (W : Type) (R : relation W) (V: variable -> W -> Prop) (kle : relation W) (PreOrder_kle : `(PreOrder kle)) :=
-   {
-    Transitive_R: `(Transitive R);
-    Subrelation_R_kle: `(subrelation R kle);
-    Subrelation_R_kle_R: (forall x y z, kle x z -> R z y -> R x y);
-    V_kle : (forall p w v, kle w v -> V p w -> V p v);
-    R_wf : well_founded (flip R)
-    }.
+(* TODO: better naming convention? *)
+Class IntuitionisticFrame (W : Type) (R : relation W).
+
+Class IntuitionisticModalFrame W R (kle : relation W) :=
+ { IntuitionisticModalFrame_IntuitionisticFrame :: IntuitionisticFrame W R;
+   IntuitionisticModalFrame_PartialOrder :: PartialOrder kle;
+   RBox : forall x y z, kle x z -> R z y -> R x y}.
+
+Class IntuitionisticK4Frame W R :=
+  { IntuitionisticK4Frame_IntuitionisticFrame ::  IntuitionisticFrame W R;
+   transitive_frame :: Transitive R}.
+
+Class StrongFrame W R (kle : relation W) :=
+  { StrongFrame_IntuitionisticModalFrame ::  IntuitionisticModalFrame W R kle;
+     strongness : subrelation R kle}.
+
+(* Class IntuitionisticTFrame `(IntuitionisticFrame) := {reflexive_frame : reflexive R}. *)
+
+Class ValuatedFrame W R (kle : relation W) (var : Type) (V: var -> W -> Prop) :=
+ { ValuatedFrame_IntuitionisticFrame :: IntuitionisticFrame W R;
+  valuation_monotonicity : forall p w v, kle w v -> V p w -> V p v}.
+
+(* TODO: should Valuation extend IntuitionisticFrame? *)
+
+(* an ISL Frame … *)
+Class ISLFrame {W} {R} {kle : relation W} {var} {V : var -> W -> Prop} :=
+ { ISL_Frame_Strong :: StrongFrame W R kle; (* is in particular a strong frame ; *)
+   ISL_Frame_K4 :: IntuitionisticK4Frame W R; (* and a K4 frame ; *)
+   ISLFrame_ValuatedFrame :: ValuatedFrame W R kle var V; (* it has a valuation *)
+   convWf :  well_founded (flip R) (* R is converse well-founded *)
+   }.
 
 Reserved Infix "⊨" (at level 80).
-Fixpoint forces `{M : IntuitionisticModalKripkeModel} (w : W) (φ : form) : Prop :=
+Fixpoint forces `{ValuatedFrame W R kle variable V} (w : W) (φ : form) : Prop :=
 match φ with
 | Var p => V p w
 | Bot => False
 | And φ ψ => w ⊨ φ /\ w ⊨ ψ
 | Or φ ψ => w ⊨ φ \/ w ⊨ ψ
-| Implies φ ψ => forall v, kle w v -> v ⊨ φ /\ v ⊨ ψ
+| Implies φ ψ => forall v, kle w v -> v ⊨ φ -> v ⊨ ψ
 | Box φ => forall v, R w v -> v ⊨ φ
 end
 where "w ⊨ φ" := (forces w φ).
 (* Note that we this is usually denoted M, w ⊨ φ, i.e. with M explicit *)
 
-Lemma persistence `{M : IntuitionisticModalKripkeModel} φ w v: kle w v -> w ⊨ φ -> v ⊨ φ.
-Proof.
+
+(* TODO: "we say that (W, ≤, R, V )
+is a model over P ⊆ Prop if the codomain of V is P(P )." *)
+
+Lemma persistence `{ISLFrame W R kle variable} φ w v: kle w v -> w ⊨ φ -> v ⊨ φ.
 Proof.
 revert w v. induction φ; intros w w' Hle Hw; simpl.
-- apply V_kle with w; auto.
+- apply valuation_monotonicity with w; auto.
 - tauto.
 - destruct Hw. eauto.
 - destruct Hw; eauto.
 - intros z Hz. apply Hw. transitivity w'; trivial.
-- intros z Hz. eapply Hw. apply Subrelation_R_kle_R with w'; trivial.
+- intros z Hz. apply Hw. now apply (RBox _ _ w').
 Qed.
 
 Definition sequent := (env * form)%type.
 
 (* slight adaptation to intuitionistic. Check equivalence *)
-Definition forces_sequent `{M : IntuitionisticModalKripkeModel} (w : W) (s : sequent) := 
+Definition forces_sequent `{ValuatedFrame W R kle variable V} (w : W) (s : sequent) := 
   let (Γ, δ) := s in (∀ φ, φ ∈ Γ -> forces w φ) -> (forces w δ).
 Notation "w '⊨s' s" := (forces_sequent w s) (at level 80).
 
-Definition sequents_equivalence (S T : list sequent) : Prop := ∀ W `(M : IntuitionisticModalKripkeModel W) (w : W), 
+
+(* TODO: prove soundness for iSL *)
+
+Definition sequents_equivalence (S T : list sequent) : Prop := ∀ W `(M : ValuatedFrame W R kle variable V) (w : W), 
   (∀ s, In s S -> forces_sequent w s) <->  (∀ t, In t T -> forces_sequent w t).
 
 (* TODO: check confusion between R and kle *)
 Definition bisimilar (p : variable) {W R V W' R' V'}
-  `{M : IntuitionisticModalKripkeModel W R V kle} (x : W) `{M' : IntuitionisticModalKripkeModel W' R' V' kle'} (x' : W') :=
+  `{M : ValuatedFrame W R kle variable V} (x : W) `{M' : ValuatedFrame W' R' kle' variable V'} (x' : W') :=
 { Z | Z x x' /\ ∀ w w', Z w w' ->
   (∀q, p ≠ q -> (V q w <-> V' q w' )) /\
   (∀ v, kle w v -> exists v', Z v v' /\ kle' w' v') /\
   (∀ v', kle' w' v' -> exists v, Z v v' /\ kle w v)
-}. (* TODO: should Z preserve R as well? *)
+}. (* TODO: should Z preserve R as well?  YES *)
 
-Lemma bisimilarity_spec p ψ `(M : IntuitionisticModalKripkeModel W R V) w `(M' : IntuitionisticModalKripkeModel W' R' V') w': `(bisimilar p w w') ->
+Lemma bisimilarity_spec p ψ `(M : ValuatedFrame W R kle variable V) w `(M' : ValuatedFrame W' R' kle' variable V') w': `(bisimilar p w w') ->
   (~ occurs_in p ψ)  -> (forces w ψ <-> forces w' ψ).
 Proof.
 revert w w'. induction ψ; intros w w' Hb Hvar; simpl in *; try tauto.
@@ -83,20 +109,100 @@ revert w w'. induction ψ; intros w w' Hb Hvar; simpl in *; try tauto.
 - split.
   + intros Hi v' Hw'v'.
       destruct Hb as [Z [Hww' HZ]]; destruct (HZ w w' Hww') as (Hv & HR & HR').
-      destruct (HR' _ (Subrelation_R_kle _ _ Hw'v')) as (v & HZv & Hwv).
+      (*
+      destruct (HR' _ (strongness _ _ Hw'v')) as (v & HZv & Hwv).
       assert(Hb' : bisimilar p v v' ) by (exists Z; split; trivial).
-      rewrite <- (IHψ v v'); try tauto. apply Hi. admit.
+      rewrite <- (IHψ v v'); try tauto. apply Hi. admit. *)
 Admitted.
 
 Require Import Coq.Program.Equality.
 
-Local Instance empty_model: IntuitionisticModalKripkeModel () (λ _ _ : (), False) (λ (_ : variable) (_ : ()), True)
+Lemma ISL_sound Γ ψ : (Provable Γ ψ) -> forall `(ISLFrame W R kle variable V), forall w, w ⊨s (Γ, ψ).
+Proof.
+intro H. dependent induction H;intros W R kle V F w; simpl; intro Hf.
+- apply (Hf p). ms.
+- apply (Hf ⊥). ms.
+- split.
+  + now apply IHProvable1.
+  + now apply IHProvable2.
+- destruct (Hf (φ ∧ ψ)); [ms|]. fold forces in *.
+  apply IHProvable. intros φ0 Hφ0. apply env_in_add in Hφ0.
+  destruct Hφ0 as [Hl|Hr]; [subst; auto|].
+  apply env_in_add in Hr.
+  destruct Hr as [Hl|Hr]; [subst; auto|].
+  apply Hf. ms.
+- left. apply IHProvable. intros. apply Hf. ms.
+- right. apply IHProvable. intros. apply Hf. ms.
+- destruct (Hf (φ ∨ ψ)); [ms| |]; fold forces in *.
+  + apply IHProvable1. intros φ0 Hφ0. apply env_in_add in Hφ0.
+      destruct Hφ0 as [Hl|Hr]; [subst; auto|]. apply Hf. ms.
+  + apply IHProvable2. intros φ0 Hφ0. apply env_in_add in Hφ0.
+      destruct Hφ0 as [Hl|Hr]; [subst; auto|]. apply Hf. ms.
+- intros v Hv Hφ. apply IHProvable. intros φ0 Hφ0. apply env_in_add in Hφ0.
+  destruct Hφ0 as [Hl|Hr]; [subst; trivial|].
+  apply persistence with w. trivial. apply Hf. ms. 
+- apply IHProvable. intros φ0 Hφ0. apply env_in_add in Hφ0.
+  destruct Hφ0 as [Hl|Hr]; [subst|apply Hf; ms].
+  apply (Hf (p → φ));[ms|reflexivity|]. apply (Hf p). ms.
+- apply IHProvable. intros φ0 Hφ0. apply env_in_add in Hφ0.
+  destruct Hφ0 as [Hl|Hr]; [subst|apply Hf; ms].
+  simpl. intros v Hv Hφ1 v' Hv' Hφ2. apply (Hf (φ1 ∧ φ2 → φ3)).
+  + ms.
+  + now transitivity v.
+  + fold forces in *. split; trivial. now apply persistence with v.
+- apply IHProvable. intros φ0 Hφ0. apply env_in_add in Hφ0.
+  destruct Hφ0 as [Hl|Hr]; [subst|].
+  + simpl. intros v Hv Hφ2. apply (Hf (φ1 ∨ φ2 → φ3)); [ms|trivial|tauto].
+  + apply env_in_add in Hr. destruct Hr as [Hl|Hr]; [subst; auto|apply Hf; ms].
+      intros v Hv Hφ1. apply (Hf (φ1 ∨ φ2 → φ3)); [ms|trivial|tauto].
+- apply IHProvable2. intros φ0 Hφ0. apply env_in_add in Hφ0.
+  destruct Hφ0 as [Hl|Hr]; [subst|apply Hf; ms].
+  apply (Hf ((φ1 → φ2) → φ3)). ms. reflexivity. apply IHProvable1.
+  intros φ0 Hφ0. apply env_in_add in Hφ0.
+  destruct Hφ0 as [Hl|Hr]; [subst|apply Hf; ms].
+  intros v Hv Hφ2. apply (Hf ((φ1 → φ2) → φ3)). ms. trivial. fold forces.
+  intros v' Hv' Hφ1. now apply persistence with v.
+- apply IHProvable2. intros φ0 Hφ0. apply env_in_add in Hφ0.
+  destruct Hφ0 as [Hl|Hr]; [subst|apply Hf; ms]. clear IHProvable2.
+  apply (Hf (□ φ1 → φ2));[ms| reflexivity|fold forces].
+  induction v as [v Hind] using (well_founded_induction convWf).
+  intros Hv. apply IHProvable1. intros φ0 Hφ0.
+  apply env_in_add in Hφ0. destruct Hφ0 as [Hl|Hr]; [subst|].
+  + apply (Hf (□ φ1 → φ2));[ms| now apply strongness |fold forces].
+      intros v' Hv'. apply Hind. trivial. now transitivity v.
+  + apply env_in_add in Hr. destruct Hr as [Hl|Hr]; [subst|].
+      * simpl. intros v' Hv'. apply Hind. trivial.  now transitivity v.
+      * apply open_boxes_spec in Hr. destruct Hr as [[Hl Hbox] | Hr].
+        -- apply persistence with w. apply strongness, Hv. apply Hf. ms.
+        -- apply (Hf (□φ0)). ms.  trivial.
+- induction w as [x Hind] using (well_founded_induction convWf).
+  intros v HRv. apply IHProvable. intros φ0 Hφ0. apply env_in_add in Hφ0.
+  destruct Hφ0 as [Hl|Hr]; [subst|].
+  + simpl. intros v' HRv'. apply IHProvable. intros φ0 Hφ0.
+       apply env_in_add in Hφ0. destruct Hφ0 as [Hl|Hr]; [subst|].
+       * simpl. apply Hind.
+        --  simpl. now apply transitive_frame with v.
+        -- intros φ0 Hφ0. apply persistence with x.
+          ++ transitivity v; now apply strongness.
+          ++ now apply Hf.
+       * apply open_boxes_spec in Hr. destruct Hr as [[Hl Hbox] | Hr].
+          -- apply persistence with x; [transitivity v; now apply strongness|]. now apply Hf.
+          -- apply Hf in Hr. apply Hr. now transitivity v.
+  + apply open_boxes_spec in Hr. destruct Hr as [[Hl Hbox] | Hr].
+      * apply persistence with x. apply strongness, HRv. now apply Hf.
+      * apply Hf in Hr. now apply Hr.
+Qed.
+
+Local Instance empty_model: ISLFrame () (λ _ _ : (), False) (λ _, (_ : ()), True)
   (λ _ _ : (), True) (Equivalence_PreOrder unit_equivalence).
 Proof. split; auto. intros x y. tauto. intro a. constructor. simpl. tauto. Qed.
 
 (* iSL:  class of finite frames where R is transitive and irreflexive. *)
 (* probably proved by generalising over sequents *)
 (* TODO: missing finiteness *)
+
+
+
 Lemma FMP_iSL_sequent Γ ψ:
   CRelationClasses.iffT
     (Provable Γ ψ)
@@ -122,3 +228,6 @@ split.
       split; eauto. intro; tauto. intuition; destruct H; simpl in *. destruct M1;  eauto. destruct M2; eauto.
       intro. constructor. simpl. tauto.
   + 
+Admitted.
+
+*)
